src/MultivariateScript.sml
@@ -7,30 +7,61 @@
 
 open HolKernel Parse boolLib bossLib;
 
-open pred_setTheory relationTheory pairTheory sumTheory listTheory;
-open prim_recTheory arithmeticTheory combinTheory;
+open bisimulationTheory listTheory finite_mapTheory;
 
-open CCSLib CCSTheory;
-open StrongEQTheory StrongEQLib StrongLawsTheory;
-open WeakEQTheory WeakEQLib WeakLawsTheory;
-open ObsCongrTheory ObsCongrLib ObsCongrLawsTheory;
+(* unused for now:
+ pred_setTheory pairTheory sumTheory prim_recTheory arithmeticTheory combinTheory;
+ *)
+
+open CCSLib CCSTheory StrongEQTheory WeakEQTheory ObsCongrTheory;
+
+(* unused for now:
+open StrongEQLib StrongLawsTheory;
+open WeakEQLib WeakLawsTheory;
+open ObsCongrLib ObsCongrLawsTheory;
 open BisimulationUptoTheory CongruenceTheory;
 open TraceTheory ExpansionTheory ContractionTheory;
+ *)
 
 val _ = new_theory "Multivariate";
 val _ = temp_loose_equality ();
 
 (* New equivalences based on listTheory.LIST_REL *)
 val _ = overload_on ("STRONG_EQL", ``LIST_REL STRONG_EQUIV``);
-val _ = overload_on (  "WEAK_EQL", ``LIST_REL STRONG_EQUIV``);
+val _ = overload_on (  "WEAK_EQL", ``LIST_REL   WEAK_EQUIV``);
 val _ = overload_on (   "OBS_EQL", ``LIST_REL    OBS_CONGR``);
 
 (* Type of all new equivalencess *)
 val _ = type_abbrev_pp ("list_simulation",
       ``:('a, 'b) CCS list -> ('a, 'b) CCS list -> bool``);
 
+(* The use of finite_mapTheory to get rid of substitution orders was
+   suggested by Konrad Slind. Easier than another Relabeling type.
+ *)
+val CCS_Subst1_def = Define `
+   (CCS_Subst1 nil         (fm :'a |-> ('a, 'b) CCS) = nil) /\
+   (CCS_Subst1 (prefix u E) fm = prefix u (CCS_Subst1 E fm)) /\
+   (CCS_Subst1 (sum E1 E2)  fm = sum (CCS_Subst1 E1 fm)
+                                     (CCS_Subst1 E2 fm)) /\
+   (CCS_Subst1 (par E1 E2)  fm = par (CCS_Subst1 E1 fm)
+                                     (CCS_Subst1 E2 fm)) /\
+   (CCS_Subst1 (restr L E)  fm = restr L (CCS_Subst1 E fm)) /\
+   (CCS_Subst1 (relab E rf) fm = relab   (CCS_Subst1 E fm) rf) /\
+   (CCS_Subst1 (var Y)      fm = if (Y IN FDOM fm) then (FAPPLY fm Y)
+                                 else (var Y)) /\
+   (CCS_Subst1 (rec Y E)    fm = if (Y IN FDOM fm) then (rec Y E)
+                                 else (rec Y (CCS_Subst1 E fm)))`;
 
+(* :('a, 'b) CCS list -> ('a |-> ('a, 'b) CCS) -> ('a, 'b) CCS list *)
+val CCS_Subst2_def = Define `
+    CCS_Subst2 ES fm = MAP (\e. CCS_Subst1 e fm) ES`;
+
+(*
+val UNIQUE_SOLUTION_OF_ROOTED_CONTRACTIONS = store_thm (
+   "UNIQUE_SOLUTION_OF_ROOTED_CONTRACTIONS",
+  ``!E. WG E ==> !P Q. OBS_contracts P (E P) /\ OBS_contracts Q (E Q) ==> OBS_CONGR P Q``,
+    ...);
+ *)
 
 val _ = export_theory ();
-val _ = print_theory_to_file "-" "MultivariateTheory.lst";
 val _ = html_theory "Multivariate";
